src/Unfolder.v
@@ -14,7 +14,7 @@ Module Type Unfolder (ST : SepTheory.SepTheory)
                      (SH : SepHeap ST SE)
                      (LEM : SepLemma.SepLemmaType ST SE).
   Module ST_EXT := SepTheory.SepTheory_Ext ST.
-  
+
   Section parametric.
     Variable types : list type.
     Variable prover : ProverT types.
@@ -28,10 +28,10 @@ Module Type Unfolder (ST : SepTheory.SepTheory)
 
     Definition hintSide := list (LEM.sepLemma types).
 
-    Parameter refineForward : hintSide -> nat -> Facts prover -> 
+    Parameter refineForward : hintSide -> nat -> Facts prover ->
       unfoldingState -> unfoldingState * bool.
 
-    Parameter refineBackward : hintSide -> nat -> Facts prover -> 
+    Parameter refineBackward : hintSide -> nat -> Facts prover ->
       unfoldingState -> unfoldingState * bool.
 
     Variable funcs : functions types.
@@ -55,7 +55,7 @@ Module Type Unfolder (ST : SepTheory.SepTheory)
     Axiom refineForward_Ok : forall hints bound facts P Q b,
       hintSideD hints ->
       ProverT_correct prover funcs ->
-      forall PC : ProverT_correct prover funcs, 
+      forall PC : ProverT_correct prover funcs,
       refineForward hints bound facts P = (Q,b) ->
       forall meta_env vars_env,
         WellTyped_env (UVars P) meta_env -> (** meta_env instantiates the uvars **)
@@ -83,13 +83,13 @@ Module Type Unfolder (ST : SepTheory.SepTheory)
     Axiom refineBackward_Ok : forall hints bound facts P Q meta_env vars_env b,
       hintSideD hints ->
       ProverT_correct prover funcs ->
-      forall PC : ProverT_correct prover funcs, 
+      forall PC : ProverT_correct prover funcs,
       refineBackward hints bound facts P = (Q,b) ->
       WellTyped_env (UVars P) meta_env -> (** meta_env instantiates the uvars **)
       WellTyped_env (Vars P) vars_env ->
       SH.WellTyped_sheap (typeof_funcs funcs) (SE.typeof_preds preds) (UVars P) (Vars P) (Heap P) = true ->
       Valid PC meta_env vars_env facts ->
-      ST.himp (ST_EXT.existsEach (skipn (length meta_env) Q.(UVars)) (fun meta_ext : env types => 
+      ST.himp (ST_EXT.existsEach (skipn (length meta_env) Q.(UVars)) (fun meta_ext : env types =>
                       (SE.sexprD funcs preds (meta_env ++ meta_ext) vars_env (SH.sheapD (Heap Q)))))
                     (SE.sexprD funcs preds meta_env vars_env (SH.sheapD (Heap P))).
   End parametric.
@@ -97,9 +97,9 @@ End Unfolder.
 
 Module Make (ST : SepTheory.SepTheory)
             (SE : SepExpr ST)
-            (Import SH : SepHeap ST SE) 
+            (Import SH : SepHeap ST SE)
             (SUBST : Instantiation.Subst)
-            (U : SyntacticUnifier SUBST) 
+            (U : SyntacticUnifier SUBST)
             (LEM : SepLemma.SepLemmaType ST SE)
             <: Unfolder ST SE SH LEM.
 
@@ -119,7 +119,7 @@ Module Make (ST : SepTheory.SepTheory)
       Definition ERROR : expr types.
       refine (Var 0).
       Qed.
-      
+
       Fixpoint openForUnification (e : expr types) : expr types :=
         match e with
           | Expr.Const _ _ => e
@@ -139,13 +139,13 @@ Module Make (ST : SepTheory.SepTheory)
       Variable G : nat.
       Variable G' : nat.
       Variable sub : SUBST.Subst types.
-      
+
       Fixpoint liftInstantiate (e : expr types) : expr types :=
         match e with
           | Expr.Const _ _ => e
-          | Var v => 
+          | Var v =>
             if NPeano.ltb v G' then (if U_or_G then UVar (v + U) else Var (v + G))
-            else let idx := U + v - G' in 
+            else let idx := U + v - G' in
                  match SUBST.Subst_lookup idx sub with
                    | None => UVar idx (** contradiction **)
                    | Some e => e
@@ -170,11 +170,11 @@ Module Make (ST : SepTheory.SepTheory)
     Record hintsPayload := {
       Forward : hintSide;
       (* Apply on the lefthand side of an implication *)
-      Backward : hintSide 
+      Backward : hintSide
       (* Apply on the righthand side *)
     }.
 
-    Definition default_hintsPayload : hintsPayload := 
+    Definition default_hintsPayload : hintsPayload :=
       {| Forward := nil
        ; Backward := nil
        |}.
@@ -188,13 +188,13 @@ Module Make (ST : SepTheory.SepTheory)
       ForwardOk : hintSideD (Forward Payload);
       BackwardOk : hintSideD (Backward Payload)
     }.
-    
+
     Theorem hintsSoundness_default : hintsSoundness default_hintsPayload.
     Proof.
       econstructor; constructor.
     Qed.
-    
-    Theorem hintsSoundness_composite l r (L : hintsSoundness l) (R : hintsSoundness r) 
+
+    Theorem hintsSoundness_composite l r (L : hintsSoundness l) (R : hintsSoundness r)
       : hintsSoundness (composite_hintsPayload l r).
     Proof.
       econstructor; simpl; eapply Folds.Forall_app; solve [ eapply ForwardOk; auto | eapply BackwardOk; auto ].
@@ -260,7 +260,7 @@ Module Make (ST : SepTheory.SepTheory)
 
     Section unfoldOne.
       Variable unify_bound : nat.
-      
+
       Variable prover : ProverT types.
       (* This prover must discharge all pure obligations of an unfolding lemma, if it is to be applied. *)
       Variable facts : Facts prover.
@@ -270,11 +270,11 @@ Module Make (ST : SepTheory.SepTheory)
 
       Fixpoint Subst_to_env U G (s : SUBST.Subst types) (ts : variables) (cur : uvar) : option (env types) :=
         match ts with
-          | nil => Some nil 
+          | nil => Some nil
           | t :: ts =>
             match SUBST.Subst_lookup cur s with
-              | None => None 
-              | Some e => 
+              | None => None
+              | Some e =>
                 match Subst_to_env U G s ts (S cur) with
                   | None => None
                   | Some env =>
@@ -291,14 +291,14 @@ Module Make (ST : SepTheory.SepTheory)
           | nil => true
           | _ :: ts => if SUBST.Subst_lookup from sub then checkAllInstantiated (S from) ts sub else false
         end.
-      
+
       (** Determine if a lemma is applicable.
        ** - [firstUVar] an index larger than the largest unification variable
        ** - [lem] is the lemma to apply
        ** - [args] is the outside
        ** - [key] is the patterns (closed by [Foralls lem]) that need to unify with [args])
        **)
-      Definition applicable U_or_G (firstUvar firstVar : nat) (lem : LEM.sepLemma types) (args key : exprs types) 
+      Definition applicable U_or_G (firstUvar firstVar : nat) (lem : LEM.sepLemma types) (args key : exprs types)
         : option (SUBST.Subst types) :=
         let numForalls := length (Lemma.Foralls lem) in
         (** NOTE: it is important that [key] is first because of the way the unification algorithm works **)
@@ -314,23 +314,23 @@ Module Make (ST : SepTheory.SepTheory)
         end.
 
       (* Returns [None] if no unfolding opportunities are found.
-       * Otherwise, return state after one unfolding. *)      
+       * Otherwise, return state after one unfolding. *)
       Definition unfoldForward (s : unfoldingState) : option unfoldingState :=
         let imps := SH.impures (Heap s) in
         let firstUvar  := length (UVars s) in
         let firstVar   := length (Vars s) in
         find (fun h =>
           match LEM.Lhs h with
-            | SE.Func f args' => 
+            | SE.Func f args' =>
               match FM.find f imps with
                 | None => None
                 | Some argss =>
                   let numForalls := length (Lemma.Foralls h) in
                   findWithRest (fun args argss =>
-                    (* We must tweak the arguments by substituting unification variables for 
+                    (* We must tweak the arguments by substituting unification variables for
                      * [forall]-quantified variables from the lemma statement. *)
                     match applicable false firstUvar firstVar h args args' with
-                      | None => None 
+                      | None => None
                       | Some subs =>
                         (* Remove the current call from the state, as we are about to replace
                          * it with a simplified set of pieces. *)
@@ -350,12 +350,12 @@ Module Make (ST : SepTheory.SepTheory)
                               ; UVars := UVars s
                               ; Heap := star_SHeap sh sh'
                               |}
-                    end                   
+                    end
                   ) argss
               end
             | _ => None
           end) hs.
-     
+
       Definition unfoldBackward (s : unfoldingState) : option unfoldingState :=
         let imps       := SH.impures (Heap s) in
         let firstUvar  := length (UVars s) in
@@ -365,12 +365,12 @@ Module Make (ST : SepTheory.SepTheory)
             | SE.Func f args' =>
               match FM.find f imps with
                 | None => None
-                | Some argss => 
+                | Some argss =>
                   findWithRest (fun args argss =>
                     match applicable true firstUvar firstVar h args args' with
                       | None => None
                       | Some subs =>
-                        (* Remove the current call from the state, as we are about to replace it with a 
+                        (* Remove the current call from the state, as we are about to replace it with a
                          * simplified set of pieces. *)
                         let impures' := FM.add f argss (impures (Heap s)) in
                         let sh := Build_SHeap impures'
@@ -380,7 +380,7 @@ Module Make (ST : SepTheory.SepTheory)
                         (* Time to hash the hint LHS, to (among other things) get the new existential variables it creates. *)
                         let (exs, sh') := hash (LEM.Lhs h) in
 
-                        (* Newly introduced variables must be replaced with unification variables, and 
+                        (* Newly introduced variables must be replaced with unification variables, and
                          * universally quantified variables must be substituted for. *)
                         let sh' := applySHeap (liftInstantiate true firstUvar firstVar (length exs) subs) sh' in
 
@@ -452,7 +452,7 @@ Module Make (ST : SepTheory.SepTheory)
         induction F; simpl; intros; think.
         { destruct x; simpl in *; unfold error in *; congruence. }
         { destruct a; simpl in *. think. apply inj_pair2 in H5. subst.
-          destruct x; simpl in *. 
+          destruct x; simpl in *.
           { inversion H0; clear H0; subst. rewrite Plus.plus_0_r. eexists; intuition eauto. }
           { rewrite Plus.plus_comm. simpl. rewrite Plus.plus_comm. eapply IHF in H1. simpl in H1. eapply H1. auto. } }
       Qed.
@@ -480,7 +480,7 @@ Module Make (ST : SepTheory.SepTheory)
       Proof.
         induction e; simpl; unfold lookupAs; intros; think;
           repeat match goal with
-                   | [ H : nth_error _ _ = Some _ |- _ ] =>  
+                   | [ H : nth_error _ _ = Some _ |- _ ] =>
                      eapply WellTyped_env_nth_error_Some in H; [ | solve [ eauto using typeof_env_WellTyped_env ] ] ; destruct H
                    | [ |- _ ] => rewrite nth_error_app_R by omega
                    | [ |- _ ] => rewrite nth_error_app_L by omega
@@ -504,7 +504,7 @@ Module Make (ST : SepTheory.SepTheory)
       Proof.
         induction e; simpl; unfold lookupAs; intros; think;
           repeat match goal with
-                   | [ H : nth_error _ _ = Some _ |- _ ] =>  
+                   | [ H : nth_error _ _ = Some _ |- _ ] =>
                      eapply WellTyped_env_nth_error_Some in H; [ | solve [ eauto using typeof_env_WellTyped_env ] ] ; destruct H
                    | [ |- _ ] => rewrite nth_error_app_R by omega
                    | [ |- _ ] => rewrite nth_error_app_L by omega
@@ -530,9 +530,9 @@ Module Make (ST : SepTheory.SepTheory)
           exprD funcs nil (G' ++ F) e t =
           exprD funcs (quant U_or_G U G') (quant (negb U_or_G) G G') (liftInstantiate U_or_G (length U) (length G) (length G') sub e) t.
       Proof.
-        induction e; repeat progress (simpl in *; unfold lookupAs in *; intros; 
+        induction e; repeat progress (simpl in *; unfold lookupAs in *; intros;
           repeat match goal with
-                   | [ H : nth_error _ _ = Some _ |- _ ] =>  
+                   | [ H : nth_error _ _ = Some _ |- _ ] =>
                      eapply WellTyped_env_nth_error_Some in H; [ | solve [ eauto using typeof_env_WellTyped_env ] ] ; destruct H
                    | [ |- _ ] => rewrite nth_error_app_R by (try rewrite typeof_env_length in *; omega)
                    | [ |- _ ] => rewrite nth_error_app_L by (try rewrite typeof_env_length in *; omega)
@@ -564,7 +564,7 @@ Module Make (ST : SepTheory.SepTheory)
       Qed.
 
       Lemma checkAllInstantiated_app : forall sub ts ts' from,
-        checkAllInstantiated from (ts ++ ts') sub = 
+        checkAllInstantiated from (ts ++ ts') sub =
         checkAllInstantiated from ts sub && checkAllInstantiated (length ts + from) ts' sub.
       Proof.
         clear. induction ts; simpl; intros; think; eauto; simpl.
@@ -583,7 +583,7 @@ Module Make (ST : SepTheory.SepTheory)
       Proof.
         clear. induction ts using rev_ind; simpl; intros; think; eauto.
         rewrite app_nil_r in *. auto.
-        rewrite checkAllInstantiated_app in H. simpl in *; think. 
+        rewrite checkAllInstantiated_app in H. simpl in *; think.
         eapply IHts; eauto. rewrite app_ass in H0. simpl in *; eauto.
         eapply is_well_typed_not_mentionsU_last. rewrite app_ass. eassumption.
         eapply SUBST.exprInstantiate_Removes. rewrite app_length. rewrite Plus.plus_comm; eauto.
@@ -595,7 +595,7 @@ Module Make (ST : SepTheory.SepTheory)
         forall u, cU <= u -> u < cU + length F -> SUBST.Subst_lookup u sub <> None.
       Proof.
         clear. induction F; simpl in *; intros; think. exfalso. omega.
-        consider (EqNat.beq_nat cU u); intros. subst. 
+        consider (EqNat.beq_nat cU u); intros. subst.
         intro. congruence. eapply IHF; eauto. omega. omega.
       Qed.
 
@@ -607,9 +607,9 @@ Module Make (ST : SepTheory.SepTheory)
         is_well_typed (typeof_funcs funcs) (quant U_or_G U G') (quant (negb U_or_G) G G')
           (liftInstantiate U_or_G (length U) (length G) (length G') sub e) t = true.
       Proof.
-        clear. induction e; repeat progress (simpl in *; unfold lookupAs in *; intros; 
+        clear. induction e; repeat progress (simpl in *; unfold lookupAs in *; intros;
           repeat match goal with
-                   | [ H : nth_error _ _ = Some _ |- _ ] =>  
+                   | [ H : nth_error _ _ = Some _ |- _ ] =>
                      eapply WellTyped_env_nth_error_Some in H; [ | solve [ eauto using typeof_env_WellTyped_env ] ] ; destruct H
                    | [ |- _ ] => rewrite nth_error_app_R by (try rewrite typeof_env_length in *; omega)
                    | [ |- _ ] => rewrite nth_error_app_L by (try rewrite typeof_env_length in *; omega)
@@ -627,17 +627,17 @@ Module Make (ST : SepTheory.SepTheory)
           cutrewrite (x + length U - length U = x); [ | omega ]. rewrite H. rewrite tvar_seqb_refl; auto.
           cutrewrite (x + length G - length G = x); [ | omega ]. rewrite H. rewrite tvar_seqb_refl; auto. }
         { consider (SUBST.Subst_lookup (length U + x - length G') sub); intros.
-          generalize H4. eapply SUBST.WellTyped_lookup in H4; eauto. destruct H4. intuition. 
+          generalize H4. eapply SUBST.WellTyped_lookup in H4; eauto. destruct H4. intuition.
           assert (is_well_typed (typeof_funcs funcs) U G e x0 = true).
           { eapply checkAllInstantiated_dropU. eauto. instantiate (1 := nil). rewrite app_nil_r. auto.
             2: eauto. 2: eauto. omega. }
           clear H7.
-          rewrite nth_error_app_R in H6 by omega. 
+          rewrite nth_error_app_R in H6 by omega.
           cutrewrite (length U + x - length G' - length U = x - length G') in H6; [ | omega ].
           rewrite H in H6; inversion H6; clear H6; subst. destruct U_or_G; simpl.
           rewrite <- app_nil_r with (l := G); eapply is_well_typed_weaken; eauto.
           rewrite <- app_nil_r with (l := U); eapply is_well_typed_weaken; eauto.
-          
+
           simpl. exfalso. apply nth_error_Some_length in H. eapply checkAllInstantiated_domain in H1.
           apply H1. eassumption. omega. omega. }
         { rewrite all2_map_1. destruct t0. clear H0. simpl in *. generalize dependent TDomain.
@@ -650,9 +650,9 @@ Module Make (ST : SepTheory.SepTheory)
         SUBST.exprInstantiate sub (openForUnification U e) = liftInstantiate quant U G 0 sub e.
       Proof.
         induction e; simpl; intros; think;
-          repeat (rewrite SUBST.exprInstantiate_Const || 
-                  rewrite SUBST.exprInstantiate_Equal || 
-                  rewrite SUBST.exprInstantiate_Func || 
+          repeat (rewrite SUBST.exprInstantiate_Const ||
+                  rewrite SUBST.exprInstantiate_Equal ||
+                  rewrite SUBST.exprInstantiate_Func ||
                   rewrite SUBST.exprInstantiate_Not ||
                   rewrite SUBST.exprInstantiate_Var ||
                   rewrite SUBST.exprInstantiate_UVar);
@@ -669,8 +669,8 @@ Module Make (ST : SepTheory.SepTheory)
         destruct r; destruct l; intuition; f_equal; auto.
       Qed.
 
-      Lemma Subst_to_env_app : forall U G sub ts ts' from, 
-        Subst_to_env U G sub (ts ++ ts') from = 
+      Lemma Subst_to_env_app : forall U G sub ts ts' from,
+        Subst_to_env U G sub (ts ++ ts') from =
         match Subst_to_env U G sub ts from , Subst_to_env U G sub ts' (length ts + from) with
           | Some l , Some r => Some (l ++ r)
           | _ , _ => None
@@ -679,9 +679,9 @@ Module Make (ST : SepTheory.SepTheory)
         induction ts; intros; simpl; think; auto.
         destruct (Subst_to_env U G sub ts' from); auto.
         cutrewrite (S (length ts + from) = length ts + S from); [ | omega ].
-        repeat match goal with 
-                 | [ |- context [ match ?X with _ => _ end ] ] => 
-                   match X with 
+        repeat match goal with
+                 | [ |- context [ match ?X with _ => _ end ] ] =>
+                   match X with
                      | match _ with _ => _ end => fail 1
                      | _ => destruct X
                    end
@@ -710,11 +710,11 @@ Module Make (ST : SepTheory.SepTheory)
           4: eauto. 2: unfold WellTyped_env in *; auto. 2: unfold WellTyped_env in *; auto.
           destruct XX. rewrite H5. eauto. }
       Qed.
-      
+
 
       (** TODO: lift this outside **)
       Lemma fold_left_2_opt_unify : forall tU tG ts args args' sub sub',
-        SUBST.Subst_WellTyped (types := types) (typeof_funcs funcs) tU tG sub -> 
+        SUBST.Subst_WellTyped (types := types) (typeof_funcs funcs) tU tG sub ->
         all2 (is_well_typed (typeof_funcs funcs) tU tG) args ts = true ->
         all2 (is_well_typed (typeof_funcs funcs) tU tG) args' ts = true ->
         fold_left_2_opt (U.exprUnify unify_bound) args args' sub = Some sub' ->
@@ -722,8 +722,8 @@ Module Make (ST : SepTheory.SepTheory)
         SUBST.Subst_Extends sub' sub /\
         map (SUBST.exprInstantiate sub') args = map (SUBST.exprInstantiate sub') args'.
       Proof.
-        clear. induction ts; destruct args; destruct args'; intros; simpl in *; think; 
-        try (congruence || solve [ intuition (eauto; reflexivity) ]). 
+        clear. induction ts; destruct args; destruct args'; intros; simpl in *; think;
+        try (congruence || solve [ intuition (eauto; reflexivity) ]).
         do 2 generalize H2. apply U.exprUnify_sound_syn in H2. intro. eapply U.exprUnify_Extends in H6.
         intro. eapply U.exprUnify_WellTyped in H7; eauto. eapply IHts in H3; eauto. destruct H3.
         intuition. etransitivity; eauto. rewrite H10. f_equal.
@@ -735,20 +735,20 @@ Module Make (ST : SepTheory.SepTheory)
         exprD funcs U G a t = Some v ->
         exprD funcs (quant ug U U') (quant ug' G G') a t = Some v.
       Proof.
-        clear; destruct ug; destruct ug'; simpl; intros; 
+        clear; destruct ug; destruct ug'; simpl; intros;
           [ | rewrite <- app_nil_r with (l := G) | rewrite <- app_nil_r with (l := U) | auto ];
-          apply exprD_weaken; auto. 
+          apply exprD_weaken; auto.
       Qed.
 
       Lemma liftInstantiate_lemmaD : forall U_or_G U G lem sub env,
         Subst_to_env U G sub (Foralls lem) (length U) = Some env ->
-        LEM.sepLemmaD funcs preds nil nil lem ->            
+        LEM.sepLemmaD funcs preds nil nil lem ->
         implyEach funcs (map (liftInstantiate U_or_G (length U) (length G) 0 sub) (Hyps lem)) U G
-                 (SE.himp funcs preds nil env (LEM.Lhs lem) (LEM.Rhs lem)). 
+                 (SE.himp funcs preds nil env (LEM.Lhs lem) (LEM.Rhs lem)).
       Proof.
         clear. destruct 2; simpl in *. eapply forallEachR_sem in H1; eauto using Subst_to_env_env.
-        eapply implyEach_sem. intros. eapply implyEach_sem in H1; eauto. 
-        
+        eapply implyEach_sem. intros. eapply implyEach_sem in H1; eauto.
+
         clear H1. unfold WellTyped_lemma in *. think. generalize dependent (Hyps lem).
         induction l; simpl; intros; auto. think. intuition. clear H4 H6.
         unfold Provable in *.
@@ -764,7 +764,10 @@ Module Make (ST : SepTheory.SepTheory)
         AllProvable funcs U G hyps.
       Proof.
         clear. induction hyps; simpl; intros; think; auto.
-        intuition; eauto. eapply Prove_correct; eauto. unfold ValidProp.
+        intuition; eauto.
+        Require Import MirrorShard.Prover.
+        eapply ProverCorrect_ProverCorrect'.
+        eapply Prove_correct; eauto. eauto. eauto. unfold ValidProp.
         eapply is_well_typed_correct; eauto using typeof_env_WellTyped_env, typeof_funcs_WellTyped_funcs.
       Qed.
 
@@ -775,9 +778,9 @@ Module Make (ST : SepTheory.SepTheory)
         SUBST.exprInstantiate sub e = e.
       Proof.
         clear; induction e; simpl in *; intros;
-          repeat (rewrite SUBST.exprInstantiate_Const || 
-            rewrite SUBST.exprInstantiate_Equal || 
-              rewrite SUBST.exprInstantiate_Func || 
+          repeat (rewrite SUBST.exprInstantiate_Const ||
+            rewrite SUBST.exprInstantiate_Equal ||
+              rewrite SUBST.exprInstantiate_Func ||
                 rewrite SUBST.exprInstantiate_Not ||
                   rewrite SUBST.exprInstantiate_Var ||
                     rewrite SUBST.exprInstantiate_UVar); think; try congruence; auto.
@@ -795,7 +798,7 @@ Module Make (ST : SepTheory.SepTheory)
 
       Lemma fromTo_length : forall b a, length (fromTo a b) = b.
       Proof.
-        clear; induction b; simpl; intros; eauto. 
+        clear; induction b; simpl; intros; eauto.
       Qed.
 
       Lemma fromTo_none_less : forall b a c,
@@ -831,12 +834,12 @@ Module Make (ST : SepTheory.SepTheory)
         checkAllInstantiated cU F sub = true ->
         forall u, u < cU -> SUBST.Subst_lookup u sub = None.
       Proof.
-        clear. intros. symmetry in H. apply beq_nat_eq in H. 
+        clear. intros. symmetry in H. apply beq_nat_eq in H.
         rewrite SUBST.Subst_size_cardinal in H. cut (~In u (SUBST.Subst_domain sub)).
         intros. consider (SUBST.Subst_lookup u sub); auto. intros. exfalso. apply H2. eapply SUBST.Subst_domain_iff. eauto.
-        
+
         apply checkAllInstantiated_perm in H0. destruct H0.
-        intro. eapply Permutation.Permutation_in in H2. 2: symmetry; eauto. apply in_app_or in H2. destruct H2. 
+        intro. eapply Permutation.Permutation_in in H2. 2: symmetry; eauto. apply in_app_or in H2. destruct H2.
         eapply fromTo_none_less in H2; eauto.
         apply Permutation.Permutation_length in H0. rewrite app_length in H0. rewrite fromTo_length in H0. rewrite <- H in H0.
         destruct x. inversion H2. unfold uvar in *. simpl in *. omega.
@@ -849,7 +852,7 @@ Module Make (ST : SepTheory.SepTheory)
         clear. induction e; simpl; intros; try solve [ think; auto ].
         think. apply nth_error_Some_length in H. auto.
         { consider (nth_error (typeof_funcs funcs) f). intros. consider (equiv_dec t (TRange t0)); think; intros.
-          clear H0. destruct t0; simpl in *. generalize dependent TDomain. revert H1. 
+          clear H0. destruct t0; simpl in *. generalize dependent TDomain. revert H1.
           induction H; try congruence; destruct TDomain; simpl in *; think; try congruence; intros.
           consider (is_well_typed (typeof_funcs funcs) U G x t); intros. apply orb_true_iff in H1. destruct H1.
           eapply H; eauto. eapply IHForall; eauto. }
@@ -868,7 +871,7 @@ Module Make (ST : SepTheory.SepTheory)
         SE.WellTyped_sexpr (typeof_funcs funcs) (SE.typeof_preds preds) nil a (LEM.Rhs b) = true.
       Proof.
         unfold LEM.WellTyped_sepConcl, LEM.Lhs, LEM.Rhs; intros.
-        match goal with 
+        match goal with
           | [ H : (if ?X then _ else _) = true |- ?Y = true /\ _ ] =>
             change X with Y in H; destruct Y
         end; intuition.
@@ -883,34 +886,34 @@ Module Make (ST : SepTheory.SepTheory)
         args = map (liftInstantiate U_or_G (length U) (length G) 0 sub) args' /\
         let (lq,lh) := hash (LEM.Lhs lem) in
         let (rq,rh) := hash (LEM.Rhs lem) in
-        ST.himp (ST_EXT.existsEach lq (fun lq => 
+        ST.himp (ST_EXT.existsEach lq (fun lq =>
                       SE.sexprD funcs preds (quant U_or_G U (rev lq)) (quant (negb U_or_G) G (rev lq))
                       (sheapD (applySHeap (liftInstantiate U_or_G (length U) (length G) (length lq) sub) lh))))
-                   (ST_EXT.existsEach rq (fun rq => 
+                   (ST_EXT.existsEach rq (fun rq =>
                       SE.sexprD funcs preds (quant U_or_G U (rev rq)) (quant (negb U_or_G) G (rev rq))
                       (sheapD (applySHeap (liftInstantiate U_or_G (length U) (length G) (length rq) sub) rh))))
-        /\ WellTyped_sheap (typeof_funcs funcs) (SE.typeof_preds preds) 
+        /\ WellTyped_sheap (typeof_funcs funcs) (SE.typeof_preds preds)
               (quant U_or_G (typeof_env U) (rev lq)) (quant (negb U_or_G) (typeof_env G) (rev lq))
                 (applySHeap (liftInstantiate U_or_G (length U) (length G) (length lq) sub) lh) = true
-        /\ WellTyped_sheap (typeof_funcs funcs) (SE.typeof_preds preds) 
+        /\ WellTyped_sheap (typeof_funcs funcs) (SE.typeof_preds preds)
               (quant U_or_G (typeof_env U) (rev rq)) (quant (negb U_or_G) (typeof_env G) (rev rq))
                 (applySHeap (liftInstantiate U_or_G (length U) (length G) (length rq) sub) rh) = true.
       Proof.
         unfold applicable; intros.
         repeat match goal with
-                 | [ H : match ?X with _ => _ end = _ |- _ ] => 
+                 | [ H : match ?X with _ => _ end = _ |- _ ] =>
                    consider X; try congruence; intros
                  | [ H : Some _ = Some _ |- _ ] => inversion H; clear H; subst
                end.
         eapply fold_left_2_opt_unify in H3. 2: apply SUBST.Subst_empty_WellTyped.
         Focus 3. eapply all2_impl. eassumption. intros. eapply is_well_typed_weaken with (u' := Foralls lem) (g' := nil).
         eassumption.
-        Focus 2. rewrite all2_map_1. eapply all2_impl. eassumption. intros. 
+        Focus 2. rewrite all2_map_1. eapply all2_impl. eassumption. intros.
         rewrite <- typeof_env_length. eapply openForUnification_typed. eauto.
         think. split.
-        { erewrite map_ext. 
+        { erewrite map_ext.
           2: intro; rewrite <- openForUnification_liftInstantiate; reflexivity.
-          think. generalize (independent_well_typed _ _ H4 H6). 
+          think. generalize (independent_well_typed _ _ H4 H6).
           revert H8. revert H1. clear. revert args'; revert TS.
           induction args; destruct args'; destruct TS; simpl in *; intros; think; try congruence.
           inversion H8. erewrite <- IHargs; eauto. f_equal. rewrite H3. symmetry. eapply exprInstantiate_noop; eauto.
@@ -926,7 +929,7 @@ Module Make (ST : SepTheory.SepTheory)
           eapply implyEach_sem in H.
           { rewrite SH.hash_denote in H. rewrite H10 in H.
             rewrite SH.hash_denote with (s := LEM.Rhs lem) in H. rewrite H9 in H. simpl in H.
-            
+
             destruct H12. clear H13. unfold WellTyped_lemma in *. think.
             unfold SE.himp in H.
             rewrite HEAP_FACTS.SEP_FACTS.himp_existsEach_ST_EXT_existsEach in H.
@@ -934,7 +937,7 @@ Module Make (ST : SepTheory.SepTheory)
             split.
             { etransitivity. etransitivity; [ | eapply H ].
               apply ST_EXT.himp_existsEach; intros.
-              
+
               erewrite <- applySHeap_wt_spec. reflexivity. intros. eauto. rewrite <- rev_length with (l := G0).
               eapply liftInstantiate_spec; eauto. rewrite <- typeof_env_app. auto.
               cutrewrite (s0 = snd (hash (LEM.Lhs lem))). rewrite typeof_env_app.
@@ -950,30 +953,30 @@ Module Make (ST : SepTheory.SepTheory)
               rewrite <- applySHeap_wt_spec. reflexivity. intros. rewrite <- rev_length with (l := G0).
               eapply liftInstantiate_spec; eauto. rewrite <- typeof_env_app. auto.
 
-              cutrewrite (s = snd (hash (LEM.Rhs lem))). rewrite typeof_env_app. rewrite typeof_env_rev. 
+              cutrewrite (s = snd (hash (LEM.Rhs lem))). rewrite typeof_env_app. rewrite typeof_env_rev.
               cutrewrite (typeof_env G0 = v). cutrewrite (v  = fst (hash (LEM.Rhs lem))).
               rewrite <- WellTyped_hash. simpl. apply Subst_to_env_typeof_env in H11. rewrite <- H11. auto.
               apply split_WellTyped_sepConcl in H13. destruct H13. auto.
 
               rewrite H9. auto. subst. reflexivity. rewrite H9. reflexivity. }
-            { 
+            {
             apply split_WellTyped_sepConcl in H13. destruct H13.
             rewrite WellTyped_hash in H14. rewrite WellTyped_hash in H13. think. simpl in *.
               rewrite (Subst_to_env_typeof_env _ _ _ _ _ H11) in *.
               split; (eapply applySHeap_typed_impl; [ | eauto ]).
               intros.
-              eapply liftInstantiate_typed with (U_or_G := U_or_G) (U := typeof_env U) (G := typeof_env G) (sub := sub) in H15. 
+              eapply liftInstantiate_typed with (U_or_G := U_or_G) (U := typeof_env U) (G := typeof_env G) (sub := sub) in H15.
               rewrite rev_length in H15. repeat rewrite typeof_env_length in H15. eapply H15. eassumption.
-              rewrite typeof_env_length. eassumption.              
+              rewrite typeof_env_length. eassumption.
               intros.
-              eapply liftInstantiate_typed with (U_or_G := U_or_G) (U := typeof_env U) (G := typeof_env G) (sub := sub) in H15. 
+              eapply liftInstantiate_typed with (U_or_G := U_or_G) (U := typeof_env U) (G := typeof_env G) (sub := sub) in H15.
               rewrite rev_length in H15. repeat rewrite typeof_env_length in H15. eapply H15. eassumption.
               rewrite typeof_env_length. eassumption. } }
           { destruct H12. clear H13. unfold WellTyped_lemma in H12. eapply allb_AllProvable; eauto.
             apply andb_true_iff in H12. destruct H12. apply split_WellTyped_sepConcl in H13. intuition.
             rewrite allb_map. eapply allb_impl. eauto. intros.
             simpl in *.
-            generalize (@liftInstantiate_typed U_or_G (typeof_env U) (typeof_env G) nil x0 tvProp sub (Foralls lem)). 
+            generalize (@liftInstantiate_typed U_or_G (typeof_env U) (typeof_env G) nil x0 tvProp sub (Foralls lem)).
             simpl. rewrite (Subst_to_env_typeof_env _ _ _ _ _ H11) in *. intro. apply H16 in H13; auto.
 
             repeat rewrite quant_nil in *. repeat rewrite typeof_env_length in *. auto.
@@ -988,27 +991,27 @@ Module Make (ST : SepTheory.SepTheory)
         args = map (liftInstantiate U_or_G (length tU) (length tG) 0 sub) args' /\
         let (lq,lh) := hash (LEM.Lhs lem) in
         let (rq,rh) := hash (LEM.Rhs lem) in
-           WellTyped_sheap (typeof_funcs funcs) (SE.typeof_preds preds) 
+           WellTyped_sheap (typeof_funcs funcs) (SE.typeof_preds preds)
              (quant U_or_G tU (rev lq)) (quant (negb U_or_G) tG (rev lq))
                 (applySHeap (liftInstantiate U_or_G (length tU) (length tG) (length lq) sub) lh) = true
-        /\ WellTyped_sheap (typeof_funcs funcs) (SE.typeof_preds preds) 
+        /\ WellTyped_sheap (typeof_funcs funcs) (SE.typeof_preds preds)
              (quant U_or_G tU (rev rq)) (quant (negb U_or_G) tG (rev rq))
                 (applySHeap (liftInstantiate U_or_G (length tU) (length tG) (length rq) sub) rh) = true.
       Proof.
         unfold applicable; intros.
         repeat match goal with
-                 | [ H : match ?X with _ => _ end = _ |- _ ] => 
+                 | [ H : match ?X with _ => _ end = _ |- _ ] =>
                    consider X; try congruence; intros
                  | [ H : Some _ = Some _ |- _ ] => inversion H; clear H; subst
                end.
         eapply fold_left_2_opt_unify in H2. 2: apply SUBST.Subst_empty_WellTyped.
         Focus 3. eapply all2_impl. eassumption. intros. eapply is_well_typed_weaken with (u' := Foralls lem) (g' := nil).
         eassumption.
-        Focus 2. rewrite all2_map_1. eapply all2_impl. eassumption. intros. 
+        Focus 2. rewrite all2_map_1. eapply all2_impl. eassumption. intros.
         eapply openForUnification_typed. eauto. intuition.
-        { erewrite map_ext. 
+        { erewrite map_ext.
           2: intro; rewrite <- openForUnification_liftInstantiate; reflexivity. apply andb_true_iff in H3.
-          think. generalize (independent_well_typed _ _ H3 H6). 
+          think. generalize (independent_well_typed _ _ H3 H6).
           revert H7. revert H0. clear. revert args'; revert TS.
           induction args; destruct args'; destruct TS; simpl in *; intros; think; try congruence.
           inversion H7. erewrite <- IHargs; eauto. f_equal. rewrite H3. symmetry. eapply exprInstantiate_noop; eauto.
@@ -1020,13 +1023,13 @@ Module Make (ST : SepTheory.SepTheory)
                    | H : _ && _ = true |- _ => apply andb_true_iff in H; destruct H
                  end.
           { unfold LEM.WellTyped_sepLemma, WellTyped_lemma in H. apply andb_true_iff in H. destruct H.
-            apply split_WellTyped_sepConcl in H10. rewrite WellTyped_hash in H10. rewrite WellTyped_hash in H10. 
+            apply split_WellTyped_sepConcl in H10. rewrite WellTyped_hash in H10. rewrite WellTyped_hash in H10.
             destruct H10. rewrite H6 in *; rewrite H8 in *. simpl in *.
             rewrite app_nil_r in *.
             split; (eapply applySHeap_typed_impl; [ | eauto ]).
             intros.
             eapply liftInstantiate_typed with (U_or_G := U_or_G) (U := tU) (G := tG) (sub := sub) in H12; eauto.
-            rewrite rev_length in *. auto. 
+            rewrite rev_length in *. auto.
             intros.
             eapply liftInstantiate_typed with (U_or_G := U_or_G) (U := tU) (G := tG) (sub := sub) in H12; eauto.
             rewrite rev_length in *. auto. } }
@@ -1035,7 +1038,7 @@ Module Make (ST : SepTheory.SepTheory)
       Lemma ST_himp_heq_L : forall U G P Q S,
         SE.heq funcs preds U G P Q ->
         ST.himp (SE.sexprD funcs preds U G Q) S ->
-        ST.himp (SE.sexprD funcs preds U G P) S. 
+        ST.himp (SE.sexprD funcs preds U G P) S.
       Proof.
         clear. intros. rewrite H. auto.
       Qed.
@@ -1059,7 +1062,7 @@ Module Make (ST : SepTheory.SepTheory)
                  | [ H : exists x, _ |- _ ] => destruct H
                  | [ H : _ /\ _ |- _ ] => destruct H
                  | [ H : context [ match ?X with _ => _ end ] |- _ ] =>
-                   (revert H; consider X; intros; try congruence) ; []                                           
+                   (revert H; consider X; intros; try congruence) ; []
                end; simpl. eexists; intuition.
       Qed.
 
@@ -1110,7 +1113,7 @@ Module Make (ST : SepTheory.SepTheory)
                  | [ H : exists x, _ |- _ ] => destruct H
                  | [ H : _ /\ _ |- _ ] => destruct H
                  | [ H : context [ match ?X with _ => _ end ] |- _ ] =>
-                   (revert H; consider X; intros; try congruence) ; []                                           
+                   (revert H; consider X; intros; try congruence) ; []
                end; simpl.
         eapply hintSideD_In in H; eauto using ForwardOk. destruct H. clear H3.
         rewrite WellTyped_sheap_eq in H0. apply andb_true_iff in H0. destruct H0.
@@ -1136,7 +1139,7 @@ Module Make (ST : SepTheory.SepTheory)
             { eapply H0 in H7. destruct v0; auto. destruct (nth_error (SE.typeof_preds preds) k); auto.
               eapply allb_impl; try eassumption. simpl; intros. eapply all2_impl; try eassumption.
               intros; rewrite <- app_nil_r with (l := UVars P). eapply is_well_typed_weaken. auto. } }
-          { eapply allb_impl; try eassumption. simpl; intros. 
+          { eapply allb_impl; try eassumption. simpl; intros.
             rewrite <- app_nil_r with (l := UVars P). eapply is_well_typed_weaken. auto. } }
         { consider (nth_error (SE.typeof_preds preds) f); try contradiction; intros.
           eapply applicable_WellTyped with (TS := t)in H4; try eassumption. intuition.
@@ -1144,7 +1147,7 @@ Module Make (ST : SepTheory.SepTheory)
           rewrite allb_app in H6; simpl in H6. apply andb_true_iff in H6. destruct H6.
           consider (all2 (is_well_typed (typeof_funcs funcs) (UVars P) (Vars P)) x1 t); try congruence.
           unfold WellTyped_lemma in *.
-          repeat match goal with 
+          repeat match goal with
                    | H : _ && _ = _ |- _ => apply andb_true_iff in H; destruct H
                  end.
           apply split_WellTyped_sepConcl in H8. destruct H8.
@@ -1170,7 +1173,7 @@ Module Make (ST : SepTheory.SepTheory)
                  | [ H : exists x, _ |- _ ] => destruct H
                  | [ H : _ /\ _ |- _ ] => destruct H
                  | [ H : context [ match ?X with _ => _ end ] |- _ ] =>
-                   (revert H; consider X; intros; try congruence) ; []                                           
+                   (revert H; consider X; intros; try congruence) ; []
                end.
         destruct P; simpl in *.
 
@@ -1183,62 +1186,62 @@ Module Make (ST : SepTheory.SepTheory)
         (SE.Func f x1)). 2: eapply H5.
           { repeat rewrite SH.sheapD_def. simpl.
             rewrite SH.impuresD_Add with (f := f) (argss := x0 ++ x2) (i := FM.remove f (FM.add f (x0 ++ x2) impures0))
-              (i' := FM.add f (x0 ++ x2) impures0). 
+              (i' := FM.add f (x0 ++ x2) impures0).
             rewrite SH.impuresD_Add with (f := f) (argss := x0 ++ x1 :: x2) (i := FM.remove f impures0).
             heq_canceler.
             symmetry. rewrite impuresD_Equiv.
             2: rewrite Equal_remove_add_remove; reflexivity. reflexivity.
             red; intros. repeat (rewrite MM.FACTS.add_o || rewrite MM.FACTS.remove_o).
             destruct (MF.FACTS.eq_dec f y). subst; auto. auto. intro. apply MM.FACTS.remove_in_iff in H8. intuition congruence.
-            red. intros. repeat (rewrite MM.FACTS.add_o || rewrite MM.FACTS.remove_o). consider (MF.FACTS.eq_dec f y); subst; auto. 
+            red. intros. repeat (rewrite MM.FACTS.add_o || rewrite MM.FACTS.remove_o). consider (MF.FACTS.eq_dec f y); subst; auto.
             intro. apply MM.FACTS.remove_in_iff in H8. intuition congruence. }
 
-          rewrite SEP_FACTS.heq_star_comm. 
+          rewrite SEP_FACTS.heq_star_comm.
           assert (SE.WellTyped_sexpr (typeof_funcs funcs) (SE.typeof_preds preds) (typeof_env meta_env) (typeof_env vars_env)
             (SE.Func (types := types) f x1) = true).
           { rewrite WellTyped_sheap_eq in WT. apply andb_true_iff in WT; intuition.
             rewrite WellTyped_impures_eq in H5. simpl in *. specialize (H5 _ _ H4).
             consider (x0 ++ x1 :: x2). intros. exfalso; destruct x0; simpl in *; congruence. intros.
-            destruct (nth_error (SE.typeof_preds preds) f); try contradiction. rewrite <- H4 in *. rewrite allb_app in H9. 
+            destruct (nth_error (SE.typeof_preds preds) f); try contradiction. rewrite <- H4 in *. rewrite allb_app in H9.
             simpl in *. think. }
           cut (SE.WellTyped_sexpr (typeof_funcs funcs) (SE.typeof_preds preds) (typeof_env meta_env) (typeof_env vars_env)
             (sheapD {| SH.impures := FM.add f (x0 ++ x2) impures0; SH.pures := pures0; SH.other := other0 |}) = true); intros.
-          
+
           eapply hintSideD_In in H2; eauto using ForwardOk.
           assert (length UVars0 = length meta_env).
           { unfold WellTyped_env in *. subst. rewrite typeof_env_length. auto. }
           rewrite H9 in *.
           simpl in H5. consider (nth_error (SE.typeof_preds preds) f); intros.
           rewrite H0 in H6. rewrite typeof_env_length in H6. eapply applicableOk in H6; [ | eauto | eauto | eauto | ].
-          Focus 2. destruct H2. unfold WellTyped_lemma in H2. think. apply split_WellTyped_sepConcl in H12. 
+          Focus 2. destruct H2. unfold WellTyped_lemma in H2. think. apply split_WellTyped_sepConcl in H12.
           destruct H12. rewrite H3 in *. simpl in *. rewrite H5 in *. eapply H12.
           { destruct H6. rewrite H3 in *. rewrite SH.hash_Func in *. rewrite H7 in *.
             rewrite ST_EXT.existsEach_nil in *.
             rewrite SH.hash_denote with (s := SE.Func f x1). rewrite SH.hash_Func.
-            unfold fst, snd, SE.existsEach. subst. 
+            unfold fst, snd, SE.existsEach. subst.
             rewrite HEAP_FACTS.applySHeap_singleton in *. simpl in *. rewrite app_nil_r in *. destruct H11. rewrite H6. clear H6.
             rewrite ST.heq_star_comm. rewrite ST_EXT.heq_pushIn. rewrite rw_skipn_app; eauto with list_length.
-            rewrite ST_EXT.existsEach_rev. split. 
+            rewrite ST_EXT.existsEach_rev. split.
             { eapply ST.heq_defn. eapply ST_EXT.heq_existsEach; intros.
               rewrite <- star_SHeap_denote. simpl. apply ST.heq_star_frame.
               { generalize dependent (sheapD {| SH.impures := FM.add f (x0 ++ x2) impures0;
                 SH.pures := pures0;
                 SH.other := other0 |}). clear; intros.
-                generalize (SEP_FACTS.sexprD_weaken_wt funcs preds meta_env nil G s vars_env). 
+                generalize (SEP_FACTS.sexprD_weaken_wt funcs preds meta_env nil G s vars_env).
                 rewrite app_nil_r. intro. rewrite H; try reflexivity. auto. }
               { rewrite rev_involutive. unfold WellTyped_env in *. subst. repeat rewrite typeof_env_length.
                 cutrewrite (length v = length (rev G)). reflexivity.
                 rewrite <- rev_length. rewrite <- H6. rewrite map_length. rewrite rev_length. reflexivity. } }
             { rewrite <- WellTyped_sheap_star. apply andb_true_iff. split.
-              repeat rewrite WellTyped_sheap_eq in *; simpl in *. apply andb_true_iff in WT; destruct WT. 
+              repeat rewrite WellTyped_sheap_eq in *; simpl in *. apply andb_true_iff in WT; destruct WT.
               apply andb_true_iff; split; auto.
               { apply WellTyped_impures_eq. intros. rewrite MM.FACTS.add_o in H13.
                 consider (MF.FACTS.eq_dec f k); subst; intros. inversion H13; clear H13; subst.
 
                 eapply WellTyped_impures_find_fst_last in H4; [ | eassumption ]. destruct (x0 ++ x2); auto.
                 destruct (nth_error (SE.typeof_preds preds) k); auto. eapply allb_impl; try eassumption.
-                rewrite H in *. rewrite H0 in *. clear; intros; simpl in *. unfold typeof_env in *. 
-                rewrite <- app_nil_r with (l := map (@projT1 _ _) meta_env). 
+                rewrite H in *. rewrite H0 in *. clear; intros; simpl in *. unfold typeof_env in *.
+                rewrite <- app_nil_r with (l := map (@projT1 _ _) meta_env).
                 eapply all2_impl; try eassumption. intros. eapply is_well_typed_weaken. auto.
                 rewrite WellTyped_impures_eq in H6. specialize (H6 _ _ H13). destruct v0; auto.
                 destruct (nth_error (SE.typeof_preds preds) k); auto.
@@ -1249,7 +1252,7 @@ Module Make (ST : SepTheory.SepTheory)
                 eapply is_well_typed_weaken. rewrite H0. rewrite H. eapply H13. }
               { destruct H11. unfold WellTyped_env in *. rewrite H. rewrite H0. rewrite typeof_env_length. apply H11. } }
             rewrite H0. rewrite typeof_env_length. reflexivity. }
-          { clear - WT H4. rewrite <- WellTyped_sheap_WellTyped_sexpr. rewrite WellTyped_sheap_eq in *. think. simpl in *. 
+          { clear - WT H4. rewrite <- WellTyped_sheap_WellTyped_sexpr. rewrite WellTyped_sheap_eq in *. think. simpl in *.
             apply andb_true_iff. split; auto. apply WellTyped_impures_eq; intros.
             rewrite MM.FACTS.add_o in H1. destruct (MF.FACTS.eq_dec f k). think.
             rewrite WellTyped_impures_eq in H. specialize (H _ _ H4). destruct x0; simpl in *. destruct x2; auto.
@@ -1258,7 +1261,7 @@ Module Make (ST : SepTheory.SepTheory)
             rewrite WellTyped_impures_eq in H. apply H; auto. }
       Qed.
 
-      Lemma ST_himp_heq_R : forall 
+      Lemma ST_himp_heq_R : forall
         (U G : env types) (P Q : SE.sexpr types)
         (S : ST.hprop),
         SE.heq funcs preds U G P Q ->
@@ -1266,7 +1269,7 @@ Module Make (ST : SepTheory.SepTheory)
         ST.himp S (SE.sexprD funcs preds U G P).
       Proof.
         clear. intros. rewrite H0. rewrite H. reflexivity.
-      Qed.          
+      Qed.
 
       Lemma unfoldBackward_WellTyped : forall facts P Q,
         unfoldBackward unify_bound prover facts hs P = Some Q ->
@@ -1280,7 +1283,7 @@ Module Make (ST : SepTheory.SepTheory)
                  | [ H : exists x, _ |- _ ] => destruct H
                  | [ H : _ /\ _ |- _ ] => destruct H
                  | [ H : context [ match ?X with _ => _ end ] |- _ ] =>
-                   (revert H; consider X; intros; try congruence) ; []                                           
+                   (revert H; consider X; intros; try congruence) ; []
                end; simpl.
         eapply hintSideD_In in H; eauto using BackwardOk. destruct H. clear H3.
         rewrite WellTyped_sheap_eq in H0. apply andb_true_iff in H0. destruct H0.
@@ -1306,7 +1309,7 @@ Module Make (ST : SepTheory.SepTheory)
             { eapply H0 in H7. destruct v0; auto. destruct (nth_error (SE.typeof_preds preds) k); auto.
               eapply allb_impl; try eassumption. simpl; intros. eapply all2_impl; try eassumption.
               intros; rewrite <- app_nil_r with (l := Vars P). eapply is_well_typed_weaken. auto. } }
-          { eapply allb_impl; try eassumption. simpl; intros. 
+          { eapply allb_impl; try eassumption. simpl; intros.
             rewrite <- app_nil_r with (l := Vars P). eapply is_well_typed_weaken. auto. } }
         { consider (nth_error (SE.typeof_preds preds) f); try contradiction; intros.
           eapply applicable_WellTyped with (TS := t)in H4; try eassumption. intuition.
@@ -1314,7 +1317,7 @@ Module Make (ST : SepTheory.SepTheory)
           rewrite allb_app in H6; simpl in H6. apply andb_true_iff in H6. destruct H6.
           consider (all2 (is_well_typed (typeof_funcs funcs) (UVars P) (Vars P)) x1 t); try congruence.
           unfold WellTyped_lemma in *.
-          repeat match goal with 
+          repeat match goal with
                    | H : _ && _ = _ |- _ => apply andb_true_iff in H; destruct H
                  end.
           apply split_WellTyped_sepConcl in H8. destruct H8.
@@ -1340,7 +1343,7 @@ Module Make (ST : SepTheory.SepTheory)
                  | [ H : exists x, _ |- _ ] => destruct H
                  | [ H : _ /\ _ |- _ ] => destruct H
                  | [ H : context [ match ?X with _ => _ end ] |- _ ] =>
-                   (revert H; consider X; intros; try congruence) ; []                                           
+                   (revert H; consider X; intros; try congruence) ; []
                end.
         destruct P; simpl in *.
 
@@ -1353,27 +1356,27 @@ Module Make (ST : SepTheory.SepTheory)
         (SE.Func f x1)). 2: eapply H5.
           { repeat rewrite SH.sheapD_def. simpl.
             rewrite SH.impuresD_Add with (f := f) (argss := x0 ++ x2) (i := FM.remove f (FM.add f (x0 ++ x2) impures0))
-              (i' := FM.add f (x0 ++ x2) impures0). 
+              (i' := FM.add f (x0 ++ x2) impures0).
             rewrite SH.impuresD_Add with (f := f) (argss := x0 ++ x1 :: x2) (i := FM.remove f impures0).
             heq_canceler.
             symmetry. rewrite impuresD_Equiv.
             2: rewrite Equal_remove_add_remove; reflexivity. reflexivity.
             red; intros. repeat (rewrite MM.FACTS.add_o || rewrite MM.FACTS.remove_o).
             destruct (MF.FACTS.eq_dec f y). subst; auto. auto. intro. apply MM.FACTS.remove_in_iff in H8. intuition congruence.
-            red. intros. repeat (rewrite MM.FACTS.add_o || rewrite MM.FACTS.remove_o). consider (MF.FACTS.eq_dec f y); subst; auto. 
+            red. intros. repeat (rewrite MM.FACTS.add_o || rewrite MM.FACTS.remove_o). consider (MF.FACTS.eq_dec f y); subst; auto.
             intro. apply MM.FACTS.remove_in_iff in H8. intuition congruence. }
 
-          rewrite SEP_FACTS.heq_star_comm. 
+          rewrite SEP_FACTS.heq_star_comm.
           assert (SE.WellTyped_sexpr (typeof_funcs funcs) (SE.typeof_preds preds) (typeof_env meta_env) (typeof_env vars_env)
             (SE.Func (types := types) f x1) = true).
           { rewrite WellTyped_sheap_eq in WT. apply andb_true_iff in WT; intuition.
             rewrite WellTyped_impures_eq in H5. simpl in *. specialize (H5 _ _ H4).
             consider (x0 ++ x1 :: x2). intros. exfalso; destruct x0; simpl in *; congruence. intros.
-            destruct (nth_error (SE.typeof_preds preds) f); try contradiction. rewrite <- H4 in *. rewrite allb_app in H9. 
+            destruct (nth_error (SE.typeof_preds preds) f); try contradiction. rewrite <- H4 in *. rewrite allb_app in H9.
             simpl in *. think. }
           cut (SE.WellTyped_sexpr (typeof_funcs funcs) (SE.typeof_preds preds) (typeof_env meta_env) (typeof_env vars_env)
             (sheapD {| SH.impures := FM.add f (x0 ++ x2) impures0; SH.pures := pures0; SH.other := other0 |}) = true); intros.
-          
+
           eapply hintSideD_In in H2; eauto using BackwardOk.
           assert (length UVars0 = length meta_env).
           { unfold WellTyped_env in *. subst. rewrite typeof_env_length. auto. }
@@ -1382,33 +1385,33 @@ Module Make (ST : SepTheory.SepTheory)
           rewrite H0 in H6. rewrite typeof_env_length in H6. eapply applicableOk in H6; [ | eauto | eauto | eauto | ].
           Focus 2. destruct H2. unfold WellTyped_lemma in H2. think.
           apply split_WellTyped_sepConcl in H12; destruct H12. rewrite H3 in *.
-          simpl in *. rewrite H5 in *. eapply H13. 
+          simpl in *. rewrite H5 in *. eapply H13.
           { destruct H6. rewrite H3 in *. rewrite SH.hash_Func in *. rewrite H7 in *.
             rewrite ST_EXT.existsEach_nil in *.
             rewrite SH.hash_denote with (s := SE.Func f x1). rewrite SH.hash_Func.
             unfold fst, snd, SE.existsEach. subst.
             rewrite applySHeap_singleton in *. simpl in *. rewrite app_nil_r in *. destruct H11. rewrite <- H6. clear H6.
             rewrite ST.heq_star_comm. rewrite ST_EXT.heq_pushIn. rewrite rw_skipn_app; eauto with list_length.
-            rewrite ST_EXT.existsEach_rev. split. 
+            rewrite ST_EXT.existsEach_rev. split.
             { eapply ST.heq_defn. rewrite rev_involutive. eapply ST_EXT.heq_existsEach; intros.
               rewrite <- star_SHeap_denote. simpl. apply ST.heq_star_frame.
               { generalize dependent (sheapD {| SH.impures := FM.add f (x0 ++ x2) impures0;
                 SH.pures := pures0;
                 SH.other := other0 |}). clear; intros.
-                generalize (SEP_FACTS.sexprD_weaken_wt funcs preds meta_env (rev G) nil s vars_env). 
+                generalize (SEP_FACTS.sexprD_weaken_wt funcs preds meta_env (rev G) nil s vars_env).
                 rewrite app_nil_r. intro. rewrite H; try reflexivity. auto. }
               { unfold WellTyped_env in *. subst. repeat rewrite map_length.
                 rewrite typeof_env_length. reflexivity. } }
             { rewrite <- WellTyped_sheap_star. apply andb_true_iff. split.
-              repeat rewrite WellTyped_sheap_eq in *; simpl in *. apply andb_true_iff in WT; destruct WT. 
+              repeat rewrite WellTyped_sheap_eq in *; simpl in *. apply andb_true_iff in WT; destruct WT.
               apply andb_true_iff; split; auto.
               { apply WellTyped_impures_eq. intros. rewrite MM.FACTS.add_o in H13.
                 consider (MF.FACTS.eq_dec f k); subst; intros. inversion H13; clear H13; subst.
 
                 eapply WellTyped_impures_find_fst_last in H4; [ | eassumption ]. destruct (x0 ++ x2); auto.
                 destruct (nth_error (SE.typeof_preds preds) k); auto. eapply allb_impl; try eassumption.
-                rewrite H in *. rewrite H0 in *. clear; intros; simpl in *. unfold typeof_env in *. 
-                rewrite <- app_nil_r with (l := map (@projT1 _ _) vars_env). 
+                rewrite H in *. rewrite H0 in *. clear; intros; simpl in *. unfold typeof_env in *.
+                rewrite <- app_nil_r with (l := map (@projT1 _ _) vars_env).
                 eapply all2_impl; try eassumption. intros. eapply is_well_typed_weaken. auto.
                 rewrite WellTyped_impures_eq in H6. specialize (H6 _ _ H13). destruct v0; auto.
                 destruct (nth_error (SE.typeof_preds preds) k); auto.
@@ -1419,7 +1422,7 @@ Module Make (ST : SepTheory.SepTheory)
                 eapply is_well_typed_weaken. rewrite H0. rewrite H. eapply H13. }
               { destruct H11. unfold WellTyped_env in *. rewrite H. rewrite H0. rewrite typeof_env_length.
                 eapply H6. } } }
-          { clear - WT H4. rewrite <- WellTyped_sheap_WellTyped_sexpr. rewrite WellTyped_sheap_eq in *. think. simpl in *. 
+          { clear - WT H4. rewrite <- WellTyped_sheap_WellTyped_sexpr. rewrite WellTyped_sheap_eq in *. think. simpl in *.
             apply andb_true_iff. split; auto. apply WellTyped_impures_eq; intros.
             rewrite MM.FACTS.add_o in H1. destruct (MF.FACTS.eq_dec f k). think.
             rewrite WellTyped_impures_eq in H. specialize (H _ _ H4). destruct x0; simpl in *. destruct x2; auto.
@@ -1427,7 +1430,7 @@ Module Make (ST : SepTheory.SepTheory)
             destruct (nth_error (SE.typeof_preds preds) k); auto. simpl in *. think. rewrite allb_app in *. simpl in H1. think; auto.
             rewrite WellTyped_impures_eq in H. apply H; auto. }
       Qed.
-      
+
       Lemma forwardLength : forall bound facts P Q r,
         forward bound facts P = (Q,r) ->
         exists vars_ext (* meta_ext *),
@@ -1457,7 +1460,7 @@ Module Make (ST : SepTheory.SepTheory)
                  | [ H : exists x, _ |- _ ] => destruct H
                  | [ H : _ /\ _ |- _ ] => destruct H
                  | [ H : context [ match ?X with _ => _ end ] |- _ ] =>
-                   (revert H; consider X; intros; try congruence) ; []                                           
+                   (revert H; consider X; intros; try congruence) ; []
                end; simpl. eexists; intuition.
       Qed.
 
@@ -1521,11 +1524,11 @@ Module Make (ST : SepTheory.SepTheory)
                        | [ H : exists x, _ |- _ ] => destruct H
                        | [ H : _ /\ _ |- _ ] => destruct H
                        | [ |- _ ] => rewrite app_ass in *
-                       | [ |- _ ] => rewrite rw_skipn_app by eauto with list_length 
+                       | [ |- _ ] => rewrite rw_skipn_app by eauto with list_length
                      end.
               rewrite ST_EXT.existsEach_app; intros.
               eapply ST_EXT.himp_existsEach. intros.
-              rewrite IHbound; try solve [  repeat match goal with 
+              rewrite IHbound; try solve [  repeat match goal with
                                                      | [ H : _ = _ |- _ ] => rewrite H
                                                    end; auto ].
               think. rewrite rw_skipn_app.
@@ -1534,14 +1537,14 @@ Module Make (ST : SepTheory.SepTheory)
               repeat rewrite app_length. rewrite typeof_env_length. subst. rewrite map_length. reflexivity.
               rewrite H5. repeat rewrite app_length. subst. rewrite H1. repeat rewrite map_length.
               unfold WellTyped_env. rewrite typeof_env_app. f_equal.
-              
+
               repeat match goal with
                        | [ H : _ = _ |- _ ] => rewrite H in *
-                     end. auto. 
+                     end. auto.
               rewrite <- app_nil_r with (l := meta_env); eapply Valid_weaken; eauto. }
             { rewrite <- WT. f_equal. rewrite H0. reflexivity. rewrite H1. reflexivity. } }
           { inversion H3; clear H3; subst. erewrite skipn_length_all.
-            rewrite ST_EXT.existsEach_nil. rewrite app_nil_r. reflexivity. 
+            rewrite ST_EXT.existsEach_nil. rewrite app_nil_r. reflexivity.
             unfold WellTyped_env in *. rewrite H1. unfold typeof_env. reflexivity. } }
       Qed.
 
@@ -1565,7 +1568,7 @@ Module Make (ST : SepTheory.SepTheory)
         WellTyped_env (Vars P) vars_env ->
         WellTyped_sheap (typeof_funcs funcs) (SE.typeof_preds preds) (UVars P) (Vars P) (Heap P) = true ->
         Valid PC meta_env vars_env facts ->
-        ST.himp (ST_EXT.existsEach (skipn (length meta_env) Q.(UVars)) (fun meta_ext : env types => 
+        ST.himp (ST_EXT.existsEach (skipn (length meta_env) Q.(UVars)) (fun meta_ext : env types =>
                    (SE.sexprD funcs preds (meta_env ++ meta_ext) vars_env (sheapD (Heap Q)))))
                 (SE.sexprD funcs preds meta_env vars_env (sheapD (Heap P))).
       Proof.
@@ -1573,7 +1576,7 @@ Module Make (ST : SepTheory.SepTheory)
         { inversion H; clear H; subst. cutrewrite (skipn (length meta_env) (UVars Q) = nil). rewrite ST_EXT.existsEach_nil.
           rewrite app_nil_r. reflexivity. rewrite H0. rewrite <- typeof_env_length. eauto with list_length. }
         { consider (unfoldBackward unify_bound prover facts hs P); intros.
-          { generalize H. 
+          { generalize H.
             eapply unfoldBackwardOk in H; eauto. intro.
             apply unfoldBackward_vars in H5. think.
             generalize (backwardLength _ _ _ H4); intro. think.
@@ -1585,13 +1588,13 @@ Module Make (ST : SepTheory.SepTheory)
             Focus 2. rewrite H7. instantiate (1 := meta_env ++ G). unfold WellTyped_env. rewrite typeof_env_app.
             f_equal. symmetry; auto.
             Focus 2. rewrite H5. apply typeof_env_WellTyped_env.
-            Focus 2. apply H6. 
+            Focus 2. apply H6.
             Focus 2. rewrite <- app_nil_r with (l := vars_env). eapply Valid_weaken; auto.
             think. rewrite <- H4.
             rewrite rw_skipn_app. apply ST_EXT.himp_existsEach. intros. rewrite app_ass. reflexivity.
             repeat rewrite app_length. rewrite typeof_env_length. subst. rewrite map_length. reflexivity.
-            rewrite <- H2. f_equal. symmetry; apply H0. symmetry; apply H1. }           
-          { inversion H4; clear H4; subst. cutrewrite (skipn (length meta_env) (UVars Q) = nil). rewrite ST_EXT.existsEach_nil. 
+            rewrite <- H2. f_equal. symmetry; apply H0. symmetry; apply H1. }
+          { inversion H4; clear H4; subst. cutrewrite (skipn (length meta_env) (UVars Q) = nil). rewrite ST_EXT.existsEach_nil.
             rewrite app_nil_r. reflexivity.  rewrite H0. rewrite <- typeof_env_length. eauto with list_length. } }
       Qed.
     End unfolder.
@@ -1610,7 +1613,7 @@ Module Make (ST : SepTheory.SepTheory)
       (us : unfoldingState types) : (unfoldingState types) * bool :=
       let '(res,n) := backward hs prover bound facts us in
       (res, negb (EqNat.beq_nat n bound)).
-    
+
     Variable funcs : functions types.
     Variable preds : SE.predicates types.
 
@@ -1643,7 +1646,7 @@ Module Make (ST : SepTheory.SepTheory)
     Theorem refineForward_Ok : forall hints bound facts P Q b,
       Forall (LEM.sepLemmaD funcs preds nil nil) hints ->
       ProverT_correct prover funcs ->
-      forall PC : ProverT_correct prover funcs, 
+      forall PC : ProverT_correct prover funcs,
       refineForward hints bound facts P = (Q,b) ->
       forall meta_env vars_env,
         WellTyped_env (UVars P) meta_env -> (** meta_env instantiates the uvars **)
@@ -1691,13 +1694,13 @@ Module Make (ST : SepTheory.SepTheory)
     Theorem refineBackward_Ok : forall hints bound facts P Q meta_env vars_env b,
       Forall (LEM.sepLemmaD funcs preds nil nil) hints ->
       ProverT_correct prover funcs ->
-      forall PC : ProverT_correct prover funcs, 
+      forall PC : ProverT_correct prover funcs,
       refineBackward hints bound facts P = (Q,b) ->
       WellTyped_env (UVars P) meta_env -> (** meta_env instantiates the uvars **)
       WellTyped_env (Vars P) vars_env ->
       SH.WellTyped_sheap (typeof_funcs funcs) (SE.typeof_preds preds) (UVars P) (Vars P) (Heap P) = true ->
       Valid PC meta_env vars_env facts ->
-      ST.himp (ST_EXT.existsEach (skipn (length meta_env) Q.(UVars)) (fun meta_ext : env types => 
+      ST.himp (ST_EXT.existsEach (skipn (length meta_env) Q.(UVars)) (fun meta_ext : env types =>
                       (SE.sexprD funcs preds (meta_env ++ meta_ext) vars_env (SH.sheapD (Heap Q)))))
                     (SE.sexprD funcs preds meta_env vars_env (SH.sheapD (Heap P))).
     Proof.
@@ -1710,4 +1713,3 @@ Module Make (ST : SepTheory.SepTheory)
   End interface.
 
 End Make.
-
